src/Bedrock/P256/PrecomputedMultiples.v
@@ -1,36 +1,55 @@
-Require Import coqutil.Datatypes.List.
-Require Import Bedrock.P256.Specs.
-Require Import coqutil.Tactics.Tactics.
-Require Import bedrock2.AbsintWordToZ coqutil.Z.Lia.
-
-Import Specs.point
-  bedrock2.Syntax
-  bedrock2.NotationsCustomEntry
-  micromega.Lia
-  ProgramLogic
-  WeakestPrecondition
-  ProgramLogic.Coercions
-  SeparationLogic
-  letexists
-  BasicC64Semantics
-  ListIndexNotations
-  SepAutoArray
-  OfListWord
-  BinInt
-  PrimeFieldTheorems
-  symmetry
-  Arith
-  Array
-  memcpy.
-
+Require Import ZArith BinInt Lia Arith PeanoNat.
 Require Import Coq.Lists.List.
 Import ListNotations.
 
+From coqutil Require Import
+  letexists
+  OfListWord
+  Word.Properties
+  Datatypes.List
+  Tactics.Tactics.
+Require Import (notations) coqutil.Map.Memory.
+
+From bedrock2 Require Import
+  Syntax
+  bottom_up_simpl
+  Array
+  SepAutoArray
+  ListIndexNotations
+  wsize
+  NotationsCustomEntry
+  ProgramLogic
+  WeakestPrecondition
+  SeparationLogic
+  AbsintWordToZ
+  ZnWords.
+Import ProgramLogic.Coercions.
+Import symmetry.
+
+From bedrock2Examples Require Import
+  memcpy.
+
+Require Import
+  PrimeFieldTheorems
+  Spec.WeierstrassCurve
+  Curves.Weierstrass.Affine
+  Curves.Weierstrass.AffineProofs
+  Curves.Weierstrass.Jacobian.Jacobian
+  Curves.Weierstrass.P256
+  Bedrock.P256.Specs.
+Import Specs.coord Specs.point.
+
+Local Open Scope string_scope.
 Local Open Scope Z_scope.
 Local Open Scope list_scope.
-Local Open Scope string_scope.
 
 #[local] Notation sizeof_point := 96%nat.
+
+(* TODO: Prove for both architectures by using a context. *)
+Require Import bedrock2.BasicC64Semantics.
+#[local] Notation width := 64%nat.
+
+Local Notation "p .+ n" := (word.add p (word.of_Z n)) (at level 50, format "p .+ n", left associativity).
 
 Definition p256_precompute_multiples := func! (p_table, p_P) {
   p256_point_set_zero(p_table);
@@ -55,18 +74,36 @@ Definition p256_precompute_multiples := func! (p_table, p_P) {
   }
 }.
 
-Import Crypto.Spec.WeierstrassCurve
-  Crypto.Curves.Weierstrass.Affine
-  Crypto.Curves.Weierstrass.AffineProofs
-  Crypto.Curves.Weierstrass.Jacobian.Jacobian
-  Curves.Weierstrass.P256
-  Crypto.Bedrock.P256.Specs
-  bedrock2.ZnWords.
-Require Import bedrock2.bottom_up_simpl.
+Definition p256_get_multiple := func! (p_out, p_table, k) {
+  unpack! sign = br_broadcast_negative(k);
+  unpack! idx = br_abs(k, sign);
 
-Import (notations) coqutil.Map.Memory.
-Local Notation "p .+ n" := (word.add p (word.of_Z n)) (at level 50, format "p .+ n", left associativity).
-Local Unset Printing Coercions.
+  (* Copy the point in positive form. *)
+  p256_select_point_from_table(p_out, p_table, idx);
+
+  (* Calculate -y, and select to copy y or -y based on the sign of k. *)
+  stackalloc 32 as p_y_opp;
+  br_memcpy(p_y_opp, p_out + $32, $32);
+  p256_coord_opp(p_y_opp);
+
+  p256_coord_select_znz(p_out + $32, sign, p_out + $32, p_y_opp)
+}.
+
+Definition p256_select_point_from_table := func! (p_out, p_table, idx) {
+  i = $0;
+  while ($17 - i) {
+    (* select condition is 0 iff i == idx *)
+    p256_point_cmov(p_out, i ^ idx, p_table + ($sizeof_point * i));
+    i = i + $1
+  }
+}.
+
+(* Puts p_z into p_out if c is zero. *)
+Definition p256_point_cmov := func! (p_out, c, p_z) {
+  p256_coord_select_znz(p_out,       c, p_z,       p_out);
+  p256_coord_select_znz(p_out + $32, c, p_z + $32, p_out + $32);
+  p256_coord_select_znz(p_out + $64, c, p_z + $64, p_out + $64)
+}.
 
 Module W.
   (* Creates 0..(n-1)*P as list. *)
@@ -81,10 +118,10 @@ Lemma length_multiples (n : nat) (A : W.point) :
   Logic.eq (List.length (W.multiples n A)) n.
 Proof. cbv [W.multiples]. rewrite length_map, length_seq; trivial. Qed.
 
-Local Ltac solve_num_pre := repeat rewrite ?length_skipn, ?length_multiples, ?length_nil,
-  ?length_firstn, ?map_length, ?length_point, ?length_app, ?length_cons in *.
+#[local] Ltac solve_num_pre := repeat rewrite ?length_skipn, ?length_multiples, ?length_nil,
+  ?length_firstn, ?map_length, ?length_point, ?length_app, ?length_cons, ?length_coord in * by (lia || ZnWords).
 
-Local Ltac solve_num := solve_num_pre; try lia; ZnWords.
+#[local] Ltac solve_num := solve_num_pre; (lia || ZnWords).
 
 Lemma multiples_nth (n : nat) (A : W.point):
   forall i : nat, i < n ->
@@ -96,7 +133,7 @@ Proof.
 Qed.
 
 #[local] Notation pointarray := (array (fun (p : word.rep) (Q : point) =>
-  sepclause_of_map ((to_bytes Q)$@p)) (word.of_Z (Z.of_nat 96))).
+  sepclause_of_map ((to_bytes Q)$@p)) (word.of_Z (Z.of_nat sizeof_point))).
 
 #[local] Notation to_affine := Jacobian.to_affine.
 #[local] Notation of_affine := Jacobian.of_affine.
@@ -110,6 +147,36 @@ Qed.
     ensures t' m := t' = t /\ exists out,
       m =* pointarray p_table out * P$@p_P * R /\
       List.Forall2 W.eq (map to_affine out) (W.multiples 17 (to_affine P))
+  }.
+
+#[export] Instance spec_of_p256_point_cmov : spec_of "p256_point_cmov" :=
+  fnspec! "p256_point_cmov" (p_out c p_z : word) / (out z : point) R,
+  { requires t m := m =* out$@p_out * z$@p_z * R;
+    ensures t' m' := t' = t /\
+      let r := if Z.eqb c 0 then z else out in (r$@p_out * z$@p_z* R)%sep m'
+  }.
+
+#[export] Instance spec_of_p256_select_point_from_table : spec_of "p256_select_point_from_table" :=
+  fnspec! "p256_select_point_from_table" p_out p_table idx / (out_old : point) (multiples : list point) R,
+  { requires t m :=
+      m =* (out_old)$@p_out * pointarray p_table multiples * R /\
+      length multiples = 17%nat /\
+      0 <= word.unsigned idx < 17;
+    ensures t' m := t' = t /\
+      m =* (nth_default (of_affine W.zero) multiples (Z.to_nat idx))$@p_out *
+          pointarray p_table multiples * R
+  }.
+
+#[export] Instance spec_of_p256_get_multiple : spec_of "p256_get_multiple" :=
+  fnspec! "p256_get_multiple" p_out p_table k / (out_old P: point) (multiples : list point) R,
+  { requires t m :=
+      m =* out_old$@p_out * pointarray p_table multiples * R /\
+      length multiples = 17%nat /\
+      Forall2 W.eq (map to_affine multiples) (W.multiples 17 (to_affine P)) /\
+      -17 < (word.signed k) < 17;
+    ensures t' m := t' = t /\ exists (out_point : point),
+      m =* out_point$@p_out * pointarray p_table multiples * R /\
+      W.eq (to_affine out_point) (W.mul (word.signed k) (to_affine P))
   }.
 
 (* Matches up word additions in a simple equation. *)
@@ -138,11 +205,221 @@ Proof.
   { eapply array_index_nat_inbounds with (n:=n). lia. }
   rewrite <- hd_skipn_nth_default.
   cancel.
-  do 2 (cancel_seps_at_indices 0%nat 0%nat; [match_up_pointers; exact eq_refl|]).
-  ecancel.
+  Morphisms.f_equiv. do 3 f_equal. solve_num.
 Qed.
 
 #[local] Ltac hyp_containing a := match goal with H : context[a] |- _ => H end.
+
+Lemma p256_point_cmov_ok : program_logic_goal_for_function! p256_point_cmov.
+Proof.
+  repeat straightline.
+
+  destruct z as (((?z_x & ?z_y) & ?z_z) & ?).
+  destruct out as (((?nz_x & ?nz_y) & ?nz_z) & ?).
+  cbv [proj1_sig proj2_sig fst snd point.to_bytes] in * |-.
+
+  repeat (let H := hyp_containing m in seprewrite_in Array.sep_eq_of_list_word_at_app H;
+    [reflexivity|solve_num|];
+  rewrite ?length_coord in H).
+  bottom_up_simpl_in_hyps.
+
+  straightline_call; ssplit; repeat straightline.
+  2,3: eexists. 1-3: ecancel_assumption. 1: solve_num.
+  straightline_call; ssplit; repeat straightline.
+  2,3: eexists. 1-3: ecancel_assumption. 1: solve_num.
+  straightline_call; ssplit; repeat straightline.
+  2,3: eexists. 1-3: ecancel_assumption. 1: solve_num.
+
+  cbv [point.to_bytes fst snd proj1_sig].
+  repeat (seprewrite Array.sep_eq_of_list_word_at_app; [reflexivity|solve_num|]).
+  rewrite !length_coord.
+  bottom_up_simpl_in_goal.
+  destruct (Z.eqb_spec c1 0); ecancel_assumption.
+Qed.
+
+Lemma p256_select_point_from_table_ok : program_logic_goal_for_function! p256_select_point_from_table.
+Proof.
+  repeat straightline.
+
+  refine ((Loops.tailrec
+    HList.polymorphic_list.nil
+    (["p_out"; "p_table"; "idx"; "i"]))
+    (fun (v:nat) t m p_out p_table idx_cur i => PrimitivePair.pair.mk (
+      let out := if idx <? v
+          then nth_default (of_affine W.zero) multiples (Z.to_nat idx)
+          else out_old in
+      m =* out$@p_out * pointarray p_table multiples * R0 /\
+      0 <= i <= 17 /\
+      idx_cur = idx /\
+      v = i :> Z
+    )
+    (fun T M _ _ _ _ => T = t /\
+      M =* (nth_default (of_affine W.zero) multiples (Z.to_nat idx))$@p_out *
+          pointarray p_table multiples * R0
+    ))
+    (fun v' v => v < v' <= 17)%nat
+    _ _ _ _ _); Loops.loop_simpl.
+  { cbv [Loops.enforce]; cbn. split; exact eq_refl. }
+  { apply PeanoNat.Nat.gt_wf. }
+
+  (* Initial state matches invariant. *)
+  { repeat straightline.
+    ssplit; cycle -1.
+    { rewrite Znat.Z2Nat.id; [exact eq_refl|ZnWords]. }
+    { case Z.ltb_spec0; try (intros; ecancel_assumption).
+      subst i. bottom_up_simpl_in_goal; lia. }
+    { ZnWords. }
+    { ZnWords. }
+    { trivial. }
+  }
+
+  (* Loop postcondition implies function postcondition. *)
+  2:{ repeat straightline. assumption. }
+
+  (* Loop body preserves invariant. *)
+  intros ?v ?t ?m ?p_out ?p_table ?idx ?i.
+  repeat straightline.
+
+  (* Handle the loop termination case. *)
+  2:{ replace v with 17%nat in * by ZnWords.
+    destruct (Z.ltb_spec0 (word.unsigned idx) (Z.of_nat 17)); [ecancel_assumption | lia].
+  }
+
+  (* Inside the loop. *)
+  assert (v < 17%nat) by ZnWords.
+
+  (* Extract the point at i0. *)
+  seprewrite_in_by (pointarray_split_nth p_table0 multiples (Z.to_nat (word.unsigned i0)))
+        ltac:(hyp_containing (m0)) solve_num.
+
+  (* constant time select of the point *)
+  straightline_call; ssplit.
+  { use_sep_assumption. cancel.
+    cancel_seps_at_indices 1%nat 1%nat. { repeat f_equal. solve_num. }
+    cbv [seps]; ecancel. }
+  repeat straightline.
+  exists (S v). split; ssplit; trivial; try solve_num.
+  2:{ split; [solve_num|]. repeat straightline. assumption. }
+
+  rewrite word.unsigned_xor_nowrap in *.
+  seprewrite_by (pointarray_split_nth p_table0 multiples (Z.to_nat (word.unsigned i0))) solve_num.
+  destruct (Z.eqb_spec (Z.lxor i0 idx) 0); rewrite Z.lxor_eq_0_iff in *.
+  (* v == idx -> select point *)
+  { destruct (Z.ltb_spec idx v); case Z.ltb_spec; intros; try lia.
+    { use_sep_assumption. cancel.
+      cancel_seps_at_indices 0%nat 1%nat. { repeat f_equal. solve_num. }
+      repeat Morphisms.f_equiv. solve_num. }
+  }
+  (* v <> idx *)
+  destruct (Z.ltb_spec idx v); case Z.ltb_spec; intros; try lia.
+  all: use_sep_assumption; cancel; repeat Morphisms.f_equiv; solve_num.
+Qed.
+
+Lemma p256_get_multiple_ok : program_logic_goal_for_function! p256_get_multiple.
+Proof.
+  repeat straightline.
+  straightline_call; trivial; repeat straightline.
+  rename x into sign.
+
+  assert (word.unsigned sign = if (word.signed k) <? 0 then (Z.ones width) else 0)
+   as Hsign. {
+    subst sign.
+    case word.lts_spec; rewrite word.signed_of_Z_nowrap by solve_num; intros;
+    case Z.ltb_spec; intros; try solve_num.
+    { exact word.unsigned_broadcast_true. }
+    { exact word.unsigned_broadcast_false. }
+  }
+
+  straightline_call; ssplit.
+  { assumption. }
+
+  repeat straightline.
+  straightline_call; ssplit.
+  { ecancel_assumption. }
+  1-3: solve_num.
+  rename x into idx.
+  let H := hyp_containing (eq (word.unsigned idx)) in rename H into Hidx.
+
+  repeat straightline.
+
+  let H := hyp_containing (@Forall2) in rename H into HForall.
+
+  eapply ListUtil.Forall2_forall_iff' with (d:=(W.zero)) (i:=(Z.to_nat (Z.abs (word.signed k)))) in HForall;
+    [|solve_num|solve_num].
+  rewrite multiples_nth in HForall by lia;
+  rewrite <- (Jacobian.to_affine_of_affine W.zero) in HForall.
+  rewrite ListUtil.map_nth_default_always in *.
+
+  rewrite Hidx in *.
+  set (nth_default (of_affine W.zero) multiples (Z.to_nat (Z.abs (word.signed k)))) as idxP in *.
+
+  (* Remember the inverted point before destructing. Gives easy access to the proof that it's on the curve. *)
+  pose (proj2_sig (Jacobian.opp idxP)) as HidxPopp.
+  cbv [Jacobian.opp proj2_sig proj1_sig] in HidxPopp.
+
+  set (idxP$@p_out) as Pmem in *.
+  destruct idxP as (((x & y) & z) & HidxP).
+  cbv [point.to_bytes fst snd proj1_sig] in Pmem. subst Pmem.
+
+  repeat (let H := hyp_containing p_out in seprewrite_in Array.sep_eq_of_list_word_at_app H;
+      [reflexivity|solve_num|]; rewrite ?length_coord in H).
+  bottom_up_simpl_in_hyps.
+
+  seprewrite_in_by array1_iff_eq_of_list_word_at ltac:(hyp_containing a) lia.
+
+  straightline_call; ssplit.
+  { ecancel_assumption. }
+  { solve_num. }
+  { rewrite length_coord; ZnWords. }
+  { ZnWords. }
+
+  repeat straightline.
+
+  straightline_call; ssplit.
+  { ecancel_assumption. }
+
+  repeat straightline.
+
+  straightline_call; ssplit.
+  { ecancel_assumption. }
+  { eexists. ecancel_assumption. }
+  { eexists. ecancel_assumption. }
+  { rewrite length_coord; ZnWords. }
+
+  repeat straightline.
+
+  (* Dealloc of a. Prep ptsto and length so straightline processes. *)
+  Require Import coqutil.Macros.symmetry.
+  pose proof (length_coord (F.opp y)).
+  seprewrite_in_by (symmetry! (Array.array1_iff_eq_of_list_word_at a)) ltac:(hyp_containing a) lia.
+
+  repeat straightline.
+
+  (* Final postcondition verification. *)
+  unshelve eexists (exist _ (x, if Z.ltb (word.signed k) 0 then F.opp y else y, z) _);
+  ssplit.
+
+  { case Z.ltb_spec; intros; assumption. }
+
+  { rewrite Hsign, Z.ones_equiv in *.
+    cbv [point.to_bytes fst snd proj1_sig] in *; cbv [seps];
+    repeat (seprewrite Array.sep_eq_of_list_word_at_app;
+        [reflexivity|solve_num|]; rewrite ?length_coord).
+    bottom_up_simpl_in_goal.
+    use_sep_assumption.
+    cancel. case Z.ltb_spec; case Z.eqb_spec; try lia; intros; ecancel. }
+
+  case Z.ltb_spec; intros.
+  { rewrite <- (Z.opp_involutive (word.signed k)).
+    rewrite ScalarMult.scalarmult_opp_l.
+    match goal with H: W.eq _ ?v |- context [W.opp (?w)] =>
+      assert (W.eq v w) as <-; [repeat Morphisms.f_equiv; lia | rewrite <- H]
+    end.
+    rewrite <-Jacobian.to_affine_opp.
+    cbv [Jacobian.opp proj1_sig].
+    reflexivity. }
+  { etransitivity; [eassumption|]. repeat Morphisms.f_equiv. lia. }
+Qed.
 
 Lemma p256_precompute_multiples_ok : program_logic_goal_for_function! p256_precompute_multiples.
 Proof.
@@ -171,13 +448,13 @@ Proof.
       (fun (v:nat) t m p_table p_P i => PrimitivePair.pair.mk (
         exists multiples todo,
         m =* (todo$@(p_table.+(Z.mul i sizeof_point)) *
-              pointarray p_table multiples * P$@p_P * R)%sep /\
+              pointarray p_table multiples * P$@p_P * R0)%sep /\
               2 <= i <= 17 /\
               v = i :> Z /\
               length todo + sizeof_point*i = 17*sizeof_point /\
               Forall2 W.eq (map to_affine multiples) (W.multiples v (to_affine P)))
       (fun T M (P_TABLE P_P I : word) => t = T /\ exists multiples : list point,
-              M =* pointarray p_table multiples * P$@p_P * R /\
+              M =* pointarray p_table multiples * P$@p_P * R0 /\
               Forall2 W.eq (map to_affine multiples) ((W.multiples 17 (Jacobian.to_affine P)))))
       (fun v' v => v < v' <= 17)%nat
       _ _ _ _ _); Loops.loop_simpl.
@@ -210,12 +487,7 @@ Proof.
     replace todo with (@nil Byte.byte) in *; cycle 1.
     { symmetry. apply length_zero_iff_nil. listZnWords. }
     rewrite ?map.of_list_word_nil in *.
-
-    (* TODO: extract this lemma to coqutil.Map.Separation *)
-    assert (sepclause_of_map_empty : Lift1Prop.iff1 (sepclause_of_map (map:=mem) Interface.map.empty) (emp True)).
-    { cbv [sepclause_of_map emp]; split; intuition congruence. }
-
-    seprewrite_in sepclause_of_map_empty ltac:(hyp_containing m0).
+    seprewrite_in @sepclause_of_map_empty ltac:(hyp_containing m0).
     eexists; ssplit; [ecancel_assumption|].
     eqapply H12. f_equal. ZnWords.
   }
