src/Bedrock/P256/Specs.v
@@ -245,6 +245,16 @@ Context {ext_spec : Semantics.ExtSpec}.
   { requires t m := m =* out$@p_out * R /\ length out = 96%nat;
     ensures t' m' := t' = t /\ m' =* (Jacobian.of_affine W.zero)$@p_out * R }.
 
+#[export] Instance spec_of_p256_coord_opp : spec_of "p256_coord_opp" :=
+  fnspec! "p256_coord_opp" p / (x : coord) R,
+  { requires t m := m =* x$@p * R;
+    ensures t' m' := t' = t /\ let x_opp := F.opp x in m' =* x_opp$@p * R }.
+
+#[export] Instance spec_of_p256_coord_selectznz  : spec_of "p256_coord_select_znz" :=
+    fnspec! "p256_coord_select_znz" (p_out c p_z p_nz : word) / out (z nz : coord) R,
+    { requires t m := m =* (out$@p_out * R) /\ m =*> nz$@p_nz /\ m =*> z$@p_z /\ length out = length z;
+      ensures t' m' := t' = t /\ let out := if Z.eqb c 0 then z else nz in (out$@p_out * R)%sep m' }.
+
 #[export] Instance spec_of_p256_coord_add : spec_of "p256_coord_add" :=
   fnspec! "p256_coord_add" p_out p_x p_y / out (x y : coord) R,
   { requires t m := m =*> x$@p_x /\ m =*> y$@p_y /\ m =* out$@p_out * R /\ length out = length x;
@@ -331,6 +341,11 @@ Context {ext_spec : Semantics.ExtSpec}.
   fnspec! "br_cmov" (c vnz vz : word) ~> r,
   { requires t m := c < 2;
     ensures t' m' := t' = t /\ m' = m /\ r = if Z.eqb c 0 then vz else vnz }.
+
+#[export] Instance spec_of_br_abs : spec_of "br_abs" :=
+  fnspec! "br_abs" (k sign_mask : word) ~> r,
+  { requires t m := word.unsigned sign_mask = if Z.ltb (word.signed k) 0 then Z.ones width else 0;
+    ensures t' m' := t' = t /\ m' = m /\ word.unsigned r = Z.abs (word.signed k) }.
 
 (* Internal intermediate functions for field arithmetic: *)
 
